very significant dev changes in lowneheim
> completely replaced the find_unifier function in formula.v by making it go through all the '01' substitutions instead of
finding just a single one recursively 
> fixed all the broken proofs in lowenheim_proof.v resulting from the above change
> broke down the final admitted lemma into 4 lower-level new admitted lemmas dealing with '01' substitutions

B_Unification/lowenheim_formula.v
@@ -10,6 +10,7 @@
 
 Require Export terms.
 
+
 Require Import List.
 Import ListNotations.
 
@@ -19,10 +20,9 @@ Import ListNotations.
 
 (** In this section we formulate Lowenheim's algorithm using the data
     structures and functions defined in the [terms] library. The final occuring
-    main function [Lowenheim_Main], takes as input a term and produces a
-    substitution that unifies the given term and it is defined towards the end
-    of the file. The substitution is said to be a most general unifier and not a
-    mere substitution, but that statement is proven in the [lowenheim_proof]
+    main function, [Lowenheim_Main], takes as input a term and produces a
+    substitution that unifies the given term. The resulting substitution is said to be a most general unifier 
+    and not a mere substitution, but that statement is proven in the [lowenheim_proof]
     file. In this section we focus on the formulation of the algorithm itself,
     without any proofs about the properties of the formula or the algorithm. *)
  
@@ -56,7 +56,7 @@ Fixpoint build_on_list_of_vars (list_var : var_set) (s : term) (sig1 : subst)
     skeleton function. The list of variables is the variables within _t_ and the
     substitions are the identical subtitution and the unifer of the term. This
     fuction will often be referred in the rest of the document as our
-    "Lownheim builder" or the "Lownheim substitution builder", etc. *)
+    "Lowenheim builder" or the "Lowenheim substitution builder" or "lowenheim builder", etc. *)
 
 Definition build_lowenheim_subst (t : term) (tau : subst) : subst :=
   build_on_list_of_vars (term_unique_vars t) t
@@ -95,40 +95,41 @@ Definition term_is_T0 (t : term) : bool :=
 
 (** Our Lownheim builder works when we provide an already existing unifier
     of the input term _t_. For our implementation to be complete we need to be
-    able to generate that initial unifier ourselves. That is why we define a
-    function to find a single ground unifier, recursively. It finds a
-    substitution with ground terms that makes the given input term equivalent to
-    [T0]. To use it, start with an empty list of replacements as the input
-    [s : subst]. *)
-
-Fixpoint rec_subst (t : term) (vars : var_set) (s : subst) : subst :=
+    able to generate that initial unifier ourselves. That is why we first need to define a
+    function to find all possible '01' substitutions (substitutions where each variable gets
+    mapped to [T0] or [T1].  *)
+  
+Fixpoint all_01_substs (vars : var_set) : list subst :=
   match vars with
-  | [] => s
-  | v' :: v =>
-    if (term_is_T0 (update_term (update_term t ((v' , T0) :: s))
-                                (rec_subst (update_term t ((v' , T0) :: s))
-                                           v ((v' , T0) :: s))))
-    then rec_subst (update_term t ((v' , T0) :: s)) v ((v' , T0) :: s)
-    else
-      if (term_is_T0 (update_term (update_term t ((v' , T1) :: s))
-                                  (rec_subst (update_term t ((v' , T1) :: s))
-                                             v ((v' , T1) :: s))))
-      then rec_subst (update_term t ((v' , T1) :: s)) v ((v' , T1) :: s)
-      else rec_subst (update_term t ((v' , T0) :: s)) v ((v' , T0) :: s)
+  | [] => [[]]
+  | v :: v' => 
+               (map (fun s => (v,T0) :: s ) (all_01_substs v'))
+                 ++
+                 (map (fun s => (v,T1) :: s) (all_01_substs v'))
   end.
 
+(*
+Compute (all_01_substs (cons 1 (cons 2 nil))).
 
-(** Next is a function to find a ground unifier of the input term, if it exists.
-    *)
+*)
+
+
+
+(** 
+Function to find an initial 'ground unifier' for our lownheim builder function. 
+It finds a substitution with ground terms that makes the given input term equivalent to
+[T0]. 
+*)
 Fixpoint find_unifier (t : term) : option subst :=
-  match update_term t (rec_subst t (term_unique_vars t) []) with
-  | T0 => Some (rec_subst t (term_unique_vars t) [])
-  | _ => None
-  end.
+ find (fun s => match (update_term t s) with
+                  | T0 => true
+                  | _ => false 
+                  end ) (all_01_substs (term_unique_vars t)). 
+
 
 
 (** Here is the main Lowenheim's formula; given a term, produce an MGU (a
-    most general substitution that makes it equivalent to T0), if there is one.
+    most general substitution that when applied on the input term, it makes it equivalent to T0), if there is one.
     Otherwise, return [None]. This function is oftern referred in the rest of
     the document as "Lowenheim Main" function or "Main Lowenheim"
     function, etc. *)
@@ -164,3 +165,11 @@ Definition apply_lowenheim_main (t : term) : term :=
   | Some s => apply_subst t s
   | None => T1
   end.
+
+(*
+
+Compute (Lowenheim_Main ((VAR 1) + (VAR 2))).
+
+Compute (apply_lowenheim_main ((VAR 1) + (VAR 2))).
+
+*)
